examples/metatheory/lambda_omega.fst
@@ -1,0 +1,56 @@
+(*
+   Copyright 2008-2015 Catalin Hritcu, Nikhil Swamy, Microsoft Research and Inria
+
+   Licensed under the Apache License, Version 2.0 (the "License");
+   you may not use this file except in compliance with the License.
+   You may obtain a copy of the License at
+
+       http://www.apache.org/licenses/LICENSE-2.0
+
+   Unless required by applicable law or agreed to in writing, software
+   distributed under the License is distributed on an "AS IS" BASIS,
+   WITHOUT WARRANTIES OR CONDITIONS OF ANY KIND, either express or implied.
+   See the License for the specific language governing permissions and
+   limitations under the License.
+*)
+
+module LambdaOmega
+
+(* Chapter 29 of TAPL: "Type Operators and Kinding" *)
+
+type var = nat
+
+type knd =
+  | KTyp
+  | KArr : knd -> knd
+
+type typ =
+  | TVar : var -> typ
+  | TLam : knd -> typ -> typ 
+  | TApp : typ -> typ
+  | TArr : typ -> typ -> typ
+
+type exp =
+  | EVar   : var -> exp
+  | EApp   : exp -> exp -> exp
+  | EAbs   : typ -> exp -> exp
+
+val is_value : exp -> Tot bool
+let is_value = is_EAbs
+
+(* Substitution *)
+
+type sub =
+  | ESub : var -> Tot exp
+  | TSub : var -> Tot typ
+
+val subst_in_exp : e:exp -> s:sub -> Tot exp (decreases e)
+val subst_eabs : s:sub -> Tot sub
+let rec subst_in_exp e s =
+  match e with
+  | EVar x -> s x
+  | EAbs t e1 -> EAbs t (subst_in_exp e1 (subst_eabs s))
+  | EApp e1 e2 -> EApp (subst_in_exp e1 s) (subst_in_exp e2 s)
+and subst_eabs s =
+  fun y -> if y = 0 then EVar y
+           else subst_in_exp (s (y-1)) sub_inc
